src/impl/TLS13.Impl.ConnectionState.LocalHandshake.fst
@@ -871,7 +871,7 @@ fn mark_sent_server_hello
   c.handshake.messages.server_hello := Some lsh;
 
   unfold (IM.is_valid_server_hello lsh sh);
-  with lsh_random lsh_key_share. _;
+  with lsh_random lsh_session_id lsh_key_share. _;
   V.to_array_pts_to lsh.IM.server_hello_key_share;
   V.to_array_pts_to c.handshake.server_key_share.bytes;
   Arr.memcpy
@@ -2314,6 +2314,7 @@ let lemma_client_hello_of_start_eq_poc
           start.CS.start_client_random
           start.CS.start_server_name
           start.CS.start_client_key_share_public
+          start.CS.start_client_random
           cs sa)
   = ()
 #pop-options
@@ -2565,7 +2566,7 @@ fn try_send_client_hello
       c.handshake.messages.client_hello_present
       c.handshake.messages.client_hello
       st0.CS.cs_model.CS.model_handshake.CS.hs_client_hello);
-    with old_client_hello_present old_l_random old_l_server_name
+    with old_client_hello_present old_l_random old_l_session_id old_l_server_name
          old_l_key_share old_l_cipher_suites old_l_signature_schemes. _;
     unfold (client_hello_metadata_exactly
       c.handshake.messages.client_hello_has_server_name
@@ -5028,7 +5029,7 @@ fn try_derive_server_shared_secret_from_private_array
     c.handshake.messages.client_hello_present
     c.handshake.messages.client_hello
     st0.CS.cs_model.CS.model_handshake.CS.hs_client_hello);
-  with ch_present ch_random ch_server_name ch_key_share ch_cipher_suites ch_signature_schemes. _;
+  with ch_present ch_random ch_session_id ch_server_name ch_key_share ch_cipher_suites ch_signature_schemes. _;
 
   let ch = Ghost.hide (Some?.v st0.CS.cs_model.CS.model_handshake.CS.hs_client_hello);
   assert (pure (st0.CS.cs_model.CS.model_handshake.CS.hs_client_hello ==
