src/impl/TLS13.Impl.ConnectionState.Network.fst
@@ -446,7 +446,7 @@ fn mark_received_server_hello
   c.handshake.messages.server_hello := Some lsh;
 
   unfold (IM.is_valid_server_hello lsh sh);
-  with lsh_random lsh_key_share. _;
+  with lsh_random lsh_session_id lsh_key_share. _;
   V.to_array_pts_to lsh.IM.server_hello_key_share;
   V.to_array_pts_to c.handshake.server_key_share.bytes;
   Arr.memcpy
@@ -660,7 +660,7 @@ fn mark_received_client_hello
     c.handshake.messages.client_hello_present
     c.handshake.messages.client_hello
     st0.CS.cs_model.CS.model_handshake.CS.hs_client_hello);
-  with old_client_hello_present old_l_random old_l_server_name
+  with old_client_hello_present old_l_random old_l_session_id old_l_server_name
        old_l_key_share old_l_cipher_suites old_l_signature_schemes. _;
   unfold (client_hello_metadata_exactly
     c.handshake.messages.client_hello_has_server_name
@@ -674,7 +674,7 @@ fn mark_received_client_hello
   assert (pure (old_ch_has_server_name == false));
 
   unfold (IM.is_valid_client_hello lch ch);
-  with lch_random lch_server_name lch_key_share
+  with lch_random lch_session_id lch_server_name lch_key_share
        lch_cipher_suites lch_signature_schemes. _;
 
   V.to_array_pts_to lch.IM.client_hello_random;
@@ -685,6 +685,15 @@ fn mark_received_client_hello
     (V.vec_to_array c.handshake.messages.client_hello.IM.client_hello_random);
   V.to_vec_pts_to lch.IM.client_hello_random;
   V.to_vec_pts_to c.handshake.messages.client_hello.IM.client_hello_random;
+
+  V.to_array_pts_to lch.IM.client_hello_session_id;
+  V.to_array_pts_to c.handshake.messages.client_hello.IM.client_hello_session_id;
+  Arr.memcpy
+    32sz
+    (V.vec_to_array lch.IM.client_hello_session_id)
+    (V.vec_to_array c.handshake.messages.client_hello.IM.client_hello_session_id);
+  V.to_vec_pts_to lch.IM.client_hello_session_id;
+  V.to_vec_pts_to c.handshake.messages.client_hello.IM.client_hello_session_id;
 
   V.to_array_pts_to lch.IM.client_hello_server_name;
   V.to_array_pts_to c.handshake.messages.client_hello.IM.client_hello_server_name;
