src/impl/TLS13.Impl.Server.Network.fst
@@ -1491,7 +1491,7 @@ fn process_network_bytes
                 (M.TlsHandshake (M.ClientHello ch))
                 raw_record_bytes));
               unfold (IM.is_valid_client_hello lch ch);
-              with random server_name key_share cipher_suites signature_schemes. _;
+              with random session_id server_name key_share cipher_suites signature_schemes. _;
               CM.lemma_cipher_suites_match_length
                 cipher_suites
                 (SZ.v lch.IM.client_hello_cipher_suites_len)
